theories/rust_typing/int_rules.v
@@ -104,47 +104,27 @@ Section typing.
     TypedBinOpVal π E L v1 (int it) n1 v2 (int it) n2 (GeOp u8) (IntOp it) (IntOp it) := λ T, i2p (type_relop_int_int E L it v1 n1 v2 n2 T (bool_decide (n1 >= n2)%Z) _ π _).
   Solve Obligations with done.
 
-  Definition arith_op_result (it : int_type) n1 n2 op : option Z :=
-    match op with
-    | AddOp => Some (n1 + n2)
-    | SubOp => Some (n1 - n2)
-    | MulOp => Some (n1 * n2)
-    | AndOp => Some (Z.land n1 n2)
-    | OrOp  => Some (Z.lor n1 n2)
-    | XorOp => Some (Z.lxor n1 n2)
-    | ShlOp => Some (n1 ≪ n2)
-    | ShrOp => Some (n1 ≫ n2)
-    | DivOp => Some (n1 `quot` n2)
-    | ModOp => Some (n1 `rem` n2)
-    | CheckedAddOp => Some (n1 + n2)
-    | CheckedSubOp => Some (n1 - n2)
-    | CheckedMulOp => Some (n1 * n2)
-    | _     => None (* Relational operators. *)
-    end.
-
   Definition arith_op_sidecond (it : int_type) (n1 n2 n : Z) op : Prop :=
     match op with
     (* these sideconditions are stronger than necessary and do not support the wrapping for unsigned unchecked ops that is allowed by the opsem *)
-    | AddOp => n ∈ it
-    | SubOp => n ∈ it
-    | MulOp => n ∈ it
+    | AddOp => True
+    | SubOp => True
+    | MulOp => True
     | AndOp => True
     | OrOp  => True
     | XorOp => True
     (* TODO: check accuracy of shifting semantics *)
     | ShlOp => 0 ≤ n2 < bits_per_int it ∧ 0 ≤ n1 ∧ n ≤ MaxInt it
     | ShrOp => 0 ≤ n2 < bits_per_int it ∧ 0 ≤ n1
-    | DivOp => n2 ≠ 0 ∧ n ∈ it
-    | ModOp => n2 ≠ 0 ∧ n ∈ it
-    | CheckedAddOp => n ∈ it
-    | CheckedSubOp => n ∈ it
-    | CheckedMulOp => n ∈ it
+    | DivOp => n2 ≠ 0
+    | ModOp => n2 ≠ 0
     | _     => True (* Relational operators. *)
     end.
 
+  (** We first define a version that wraps the result and has few sideconditions *)
   Lemma type_arithop_int_int E L π it v1 n1 v2 n2 (T : typed_val_expr_cont_t) n op:
     int_arithop_result it n1 n2 op = Some n →
-    (⌜n1 ∈ it⌝ -∗ ⌜n2 ∈ it⌝ -∗ ⌜arith_op_sidecond it n1 n2 n op⌝ ∗ T L π (i2v n it) Z (int it) n) ⊢
+    (⌜n1 ∈ it⌝ -∗ ⌜n2 ∈ it⌝ -∗ ⌜arith_op_sidecond it n1 n2 n op⌝ ∗ T L π (i2v (wrap_to_it n it) it) Z (int it) (wrap_to_it n it)) ⊢
       typed_bin_op E L v1 (v1 ◁ᵥ{π} n1 @ int it) v2 (v2 ◁ᵥ{π} n2 @ int it) op (IntOp it) (IntOp it) T.
   Proof.
     rewrite /ty_own_val/=.
@@ -159,44 +139,151 @@ Section typing.
     rewrite /ty_own_val/=.
     iPureIntro. split; first by apply: val_to_of_Z. done.
   Qed.
+
+  (** Now we derive a version that gets rid of the wrapping at the cost of additional sideconditions *)
+  Definition int_arithop_in_range (it : int_type) (n : Z) op : Prop :=
+    match op with
+    (* these sideconditions are stronger than necessary and do not support the wrapping for unsigned unchecked ops that is allowed by the opsem *)
+    | AddOp => n ∈ it
+    | SubOp => n ∈ it
+    | MulOp => n ∈ it
+    | AndOp => True
+    | OrOp  => True
+    | XorOp => True
+    (* TODO: check accuracy of shifting semantics *)
+    | ShlOp => True
+    | ShrOp => True
+    | DivOp => n ∈ it
+    | ModOp => n ∈ it
+    | _     => True (* Relational operators. *)
+    end.
+
+  Lemma bitwise_op_result_in_range op bop (it : int_type) n1 n2 :
+    (0 ≤ n1 → 0 ≤ n2 → 0 ≤ op n1 n2) →
+    bool_decide (op n1 n2 < 0) = bop (bool_decide (n1 < 0)) (bool_decide (n2 < 0)) →
+    (∀ k, Z.testbit (op n1 n2) k = bop (Z.testbit n1 k) (Z.testbit n2 k)) →
+    n1 ∈ it → n2 ∈ it → op n1 n2 ∈ it.
+  Proof.
+    move => Hnonneg Hsign Htestbit.
+    rewrite !int_elem_of_it_iff.
+    rewrite /elem_of /int_elem_of_it /min_int /max_int.
+    have ? := bits_per_int_gt_0 it.
+    destruct (it_signed it).
+    - rewrite /int_half_modulus.
+      move ? : (bits_per_int it - 1) => k.
+      have Hb : ∀ n, -2^k ≤ n ≤ 2^k - 1 ↔ ∀ l, k ≤ l → Z.testbit n l = bool_decide (n < 0).
+      { move => ?. rewrite -Z.bounded_iff_bits; lia. }
+      move => /Hb Hn1 /Hb Hn2.
+      apply Hb => l Hl.
+      by rewrite Htestbit Hsign Hn1 ?Hn2.
+    - rewrite /int_modulus.
+      move ? : (bits_per_int it) => k.
+      have Hb : ∀ n, 0 ≤ n → n ≤ 2^k - 1 ↔ ∀ l, k ≤ l → Z.testbit n l = bool_decide (n < 0).
+      { move => ??. rewrite bool_decide_false -?Z.bounded_iff_bits_nonneg; lia. }
+      move => [Hn1 /Hb HN1] [Hn2 /Hb HN2].
+      have Hn := Hnonneg Hn1 Hn2.
+      split; first done.
+      apply (Hb _ Hn) => l Hl.
+      by rewrite Htestbit HN1 ?HN2.
+  Qed.
+
+  Lemma int_arithop_result_in_range (it : int_type) (n1 n2 n : Z) op :
+    n1 ∈ it → n2 ∈ it →
+    int_arithop_result it n1 n2 op = Some n →
+    int_arithop_sidecond it n1 n2 n op →
+    int_arithop_in_range it n op →
+    n ∈ it.
+  Proof.
+    move => Hn1 Hn2 Hn Hsc Hran.
+    destruct op => //=; simpl in Hsc, Hran, Hn; destruct_and? => //.
+    all: inversion Hn; simplify_eq.
+    - apply (bitwise_op_result_in_range Z.land andb) => //.
+      + rewrite Z.land_nonneg; naive_solver.
+      + repeat case_bool_decide; try rewrite -> Z.land_neg in *; naive_solver.
+      + by apply Z.land_spec.
+    - apply (bitwise_op_result_in_range Z.lor orb) => //.
+      + by rewrite Z.lor_nonneg.
+      + repeat case_bool_decide; try rewrite -> Z.lor_neg in *; naive_solver.
+      + by apply Z.lor_spec.
+    - apply (bitwise_op_result_in_range Z.lxor xorb) => //.
+      + by rewrite Z.lxor_nonneg.
+      + have Hn : ∀ n, bool_decide (n < 0) = negb (bool_decide (0 ≤ n)).
+        { intros. repeat case_bool_decide => //; lia. }
+        rewrite !Hn.
+        repeat case_bool_decide; try rewrite -> Z.lxor_nonneg in *; naive_solver.
+      + by apply Z.lxor_spec.
+    - rewrite !int_elem_of_it_iff.
+      split.
+      + trans 0; [ apply min_int_le_0 | by apply Z.shiftl_nonneg ].
+      + done.
+    - rewrite !int_elem_of_it_iff. rewrite int_elem_of_it_iff in Hn1, Hn2.
+      split.
+      + trans 0; [ apply min_int_le_0 | by apply Z.shiftr_nonneg ].
+      + destruct Hn1.
+        trans n1; last done. rewrite Z.shiftr_div_pow2; last by lia.
+        apply Z.div_le_upper_bound. { apply Z.pow_pos_nonneg => //. }
+        rewrite -{1}(Z.mul_1_l n1). apply Z.mul_le_mono_nonneg_r => //.
+        rewrite -(Z.pow_0_r 2). apply Z.pow_le_mono_r; lia.
+  Qed.
+
+  Lemma type_arithop_int_int_nowrap E L π it v1 n1 v2 n2 (T : typed_val_expr_cont_t) n op:
+    int_arithop_result it n1 n2 op = Some n →
+    (⌜n1 ∈ it⌝ -∗ ⌜n2 ∈ it⌝ -∗ ⌜arith_op_sidecond it n1 n2 n op⌝ ∗ ⌜int_arithop_in_range it n op⌝ ∗ T L π (i2v n it) Z (int it) n) ⊢
+      typed_bin_op E L v1 (v1 ◁ᵥ{π} n1 @ int it) v2 (v2 ◁ᵥ{π} n2 @ int it) op (IntOp it) (IntOp it) T.
+  Proof.
+    rewrite /ty_own_val/=.
+    iIntros "%Hop HT [%Hv1 %] [%Hv2 _] %Φ #CTX #HE HL HΦ".
+    rewrite !int_elem_of_it_iff.
+    iDestruct ("HT" with "[] []" ) as (Hsc Hran) "HT".
+    1-2: iPureIntro; by apply: val_to_Z_in_range.
+    assert (int_arithop_sidecond it n1 n2 n op).
+    { move: Hsc. rewrite /int_arithop_sidecond /arith_op_sidecond. destruct op; rewrite ?int_elem_of_it_iff ?MaxInt_eq; done. }
+    iApply wp_int_arithop; [done..| ].
+
+    iIntros (v Hv) "!> Hcred".
+    assert (wrap_to_it n it = n) as Heq.
+    { rewrite wrap_to_it_id; [done | apply int_elem_of_it_iff].
+      eapply int_arithop_result_in_range.
+      - apply int_elem_of_it_iff; eapply val_to_Z_in_range; apply Hv1.
+      - apply int_elem_of_it_iff; eapply val_to_Z_in_range; apply Hv2.
+      - done.
+      - done.
+      - done. }
+
+    rewrite Heq in Hv. rewrite /i2v Hv/=.
+    iApply ("HΦ" with "HL [] HT").
+    rewrite /ty_own_val/=.
+    iPureIntro. split; first by apply: val_to_of_Z. done.
+  Qed.
   Global Program Instance type_add_int_int_inst E L π it v1 n1 v2 n2:
-    TypedBinOpVal π E L v1 (int it) n1 v2 (int it) n2 AddOp (IntOp it) (IntOp it) := λ T, i2p (type_arithop_int_int E L π it v1 n1 v2 n2 T (n1 + n2) _ _).
+    TypedBinOpVal π E L v1 (int it) n1 v2 (int it) n2 AddOp (IntOp it) (IntOp it) := λ T, i2p (type_arithop_int_int_nowrap E L π it v1 n1 v2 n2 T (n1 + n2) _ _).
   Next Obligation. done. Qed.
   Global Program Instance type_sub_int_int_inst E L π it v1 n1 v2 n2:
-    TypedBinOpVal π E L v1 (int it) n1 v2 (int it) n2 SubOp (IntOp it) (IntOp it) := λ T, i2p (type_arithop_int_int E L π it v1 n1 v2 n2 T (n1 - n2) _ _).
+    TypedBinOpVal π E L v1 (int it) n1 v2 (int it) n2 SubOp (IntOp it) (IntOp it) := λ T, i2p (type_arithop_int_int_nowrap E L π it v1 n1 v2 n2 T (n1 - n2) _ _).
   Next Obligation. done. Qed.
   Global Program Instance type_mul_int_int_inst E L π it v1 n1 v2 n2:
-    TypedBinOpVal π E L v1 (int it) n1 v2 (int it) n2 MulOp (IntOp it) (IntOp it) := λ T, i2p (type_arithop_int_int E L π it v1 n1 v2 n2 T (n1 * n2) _ _).
-  Next Obligation. done. Qed.
-  Global Program Instance type_checked_add_int_int_inst E L π it v1 n1 v2 n2:
-    TypedBinOpVal π E L v1 (int it) n1 v2 (int it) n2 CheckedAddOp (IntOp it) (IntOp it) := λ T, i2p (type_arithop_int_int E L π it v1 n1 v2 n2 T (n1 + n2) _ _).
-  Next Obligation. done. Qed.
-  Global Program Instance type_checked_sub_int_int_inst E L π it v1 n1 v2 n2:
-    TypedBinOpVal π E L v1 (int it) n1 v2 (int it) n2 CheckedSubOp (IntOp it) (IntOp it) := λ T, i2p (type_arithop_int_int E L π it v1 n1 v2 n2 T (n1 - n2) _ _).
-  Next Obligation. done. Qed.
-  Global Program Instance type_checked_mul_int_int_inst E L π it v1 n1 v2 n2:
-    TypedBinOpVal π E L v1 (int it) n1 v2 (int it) n2 CheckedMulOp (IntOp it) (IntOp it) := λ T, i2p (type_arithop_int_int E L π it v1 n1 v2 n2 T (n1 * n2) _ _).
+    TypedBinOpVal π E L v1 (int it) n1 v2 (int it) n2 MulOp (IntOp it) (IntOp it) := λ T, i2p (type_arithop_int_int_nowrap E L π it v1 n1 v2 n2 T (n1 * n2) _ _).
   Next Obligation. done. Qed.
   Global Program Instance type_div_int_int_inst E L π it v1 n1 v2 n2:
-    TypedBinOpVal π E L v1 (int it) n1 v2 (int it) n2 DivOp (IntOp it) (IntOp it) := λ T, i2p (type_arithop_int_int E L π it v1 n1 v2 n2 T (n1 `quot` n2) _ _).
+    TypedBinOpVal π E L v1 (int it) n1 v2 (int it) n2 DivOp (IntOp it) (IntOp it) := λ T, i2p (type_arithop_int_int_nowrap E L π it v1 n1 v2 n2 T (n1 `quot` n2) _ _).
   Next Obligation. done. Qed.
   Global Program Instance type_mod_int_int_inst E L π it v1 n1 v2 n2:
-    TypedBinOpVal π E L v1 (int it) n1 v2 (int it) n2 ModOp (IntOp it) (IntOp it) := λ T, i2p (type_arithop_int_int E L π it v1 n1 v2 n2 T (n1 `rem` n2) _ _).
+    TypedBinOpVal π E L v1 (int it) n1 v2 (int it) n2 ModOp (IntOp it) (IntOp it) := λ T, i2p (type_arithop_int_int_nowrap E L π it v1 n1 v2 n2 T (n1 `rem` n2) _ _).
   Next Obligation. done. Qed.
   Global Program Instance type_and_int_int_inst E L π it v1 n1 v2 n2:
-    TypedBinOpVal π E L v1 (int it) n1 v2 (int it) n2 AndOp (IntOp it) (IntOp it) := λ T, i2p (type_arithop_int_int E L π it v1 n1 v2 n2 T (Z.land n1 n2) _ _).
+    TypedBinOpVal π E L v1 (int it) n1 v2 (int it) n2 AndOp (IntOp it) (IntOp it) := λ T, i2p (type_arithop_int_int_nowrap E L π it v1 n1 v2 n2 T (Z.land n1 n2) _ _).
   Next Obligation. done. Qed.
   Global Program Instance type_or_int_int_inst E L π it v1 n1 v2 n2:
-    TypedBinOpVal π E L v1 (int it) n1 v2 (int it) n2 OrOp (IntOp it) (IntOp it) := λ T, i2p (type_arithop_int_int E L π it v1 n1 v2 n2 T (Z.lor n1 n2) _ _).
+    TypedBinOpVal π E L v1 (int it) n1 v2 (int it) n2 OrOp (IntOp it) (IntOp it) := λ T, i2p (type_arithop_int_int_nowrap E L π it v1 n1 v2 n2 T (Z.lor n1 n2) _ _).
   Next Obligation. done. Qed.
   Global Program Instance type_xor_int_int_inst E L π it v1 n1 v2 n2:
-    TypedBinOpVal π E L v1 (int it) n1 v2 (int it) n2 XorOp (IntOp it) (IntOp it) := λ T, i2p (type_arithop_int_int E L π it v1 n1 v2 n2 T (Z.lxor n1 n2) _ _).
+    TypedBinOpVal π E L v1 (int it) n1 v2 (int it) n2 XorOp (IntOp it) (IntOp it) := λ T, i2p (type_arithop_int_int_nowrap E L π it v1 n1 v2 n2 T (Z.lxor n1 n2) _ _).
   Next Obligation. done. Qed.
   Global Program Instance type_shl_int_int_inst E L π it v1 n1 v2 n2:
-    TypedBinOpVal π E L v1 (int it) n1 v2 (int it) n2 ShlOp (IntOp it) (IntOp it) := λ T, i2p (type_arithop_int_int E L π it v1 n1 v2 n2 T (n1 ≪ n2) _ _).
+    TypedBinOpVal π E L v1 (int it) n1 v2 (int it) n2 ShlOp (IntOp it) (IntOp it) := λ T, i2p (type_arithop_int_int_nowrap E L π it v1 n1 v2 n2 T (n1 ≪ n2) _ _).
   Next Obligation. done. Qed.
   Global Program Instance type_shr_int_int_inst E L π it v1 n1 v2 n2:
-    TypedBinOpVal π E L v1 (int it) n1 v2 (int it) n2 ShrOp (IntOp it) (IntOp it) := λ T, i2p (type_arithop_int_int E L π it v1 n1 v2 n2 T (n1 ≫ n2) _ _).
+    TypedBinOpVal π E L v1 (int it) n1 v2 (int it) n2 ShrOp (IntOp it) (IntOp it) := λ T, i2p (type_arithop_int_int_nowrap E L π it v1 n1 v2 n2 T (n1 ≫ n2) _ _).
   Next Obligation. done. Qed.
 
   Inductive destruct_hint_switch_int :=
@@ -226,6 +313,7 @@ Section typing.
   Global Instance type_switch_int_inst π E L n v it : TypedSwitch π E L v _ (int it) n it :=
     λ m ss def fn R ϝ, i2p (type_switch_int π E L n it m ss def fn R ϝ v).
 
+
   Lemma type_neg_int π E L n it v (T : typed_un_op_cont_t) :
     (⌜n ∈ it⌝ -∗ ⌜it.(it_signed)⌝ ∗ ⌜n ≠ MinInt it⌝ ∗ T L π (i2v (-n) it) _ (int it) (-n))
     ⊢ typed_un_op E L v (v ◁ᵥ{π} n @ int it)%I (NegOp) (IntOp it) T.
@@ -238,8 +326,12 @@ Section typing.
       unfold elem_of, int_elem_of_it, max_int, min_int in *.
       destruct it as [?[]] => //; simpl in *; lia.
     }
+    assert (-n ∈ it) as Helem.
+    { apply int_elem_of_it_iff. by eapply val_of_Z_in_range. }
     rewrite /i2v Hv'/=.
-    iApply wp_neg_int => //. iNext. iIntros "Hcred".
+    iApply wp_neg_int => //.
+    { rewrite wrap_to_it_id; first done. apply int_elem_of_it_iff => //. }
+    iNext. iIntros "Hcred".
     iApply ("HΦ" with "HL [] HT").
     rewrite /ty_own_val/=.
     iPureIntro. split; last done. by apply: val_to_of_Z.
@@ -248,7 +340,6 @@ Section typing.
     TypedUnOpVal π E L v (int it)%I n NegOp (IntOp it) :=
     λ T, i2p (type_neg_int π E L n it v T).
 
-  (*(if it_signed it then Z.lnot n else Z_lunot (bits_per_int it) n)*)
   Lemma type_not_int π E L n it v (T : typed_un_op_cont_t) :
     (⌜n ∈ it⌝ -∗ T L π (i2v ((if it_signed it then Z.lnot n else Z_lunot (bits_per_int it) n)) it) _ (int it) ((if it_signed it then Z.lnot n else Z_lunot (bits_per_int it) n)))
     ⊢ typed_un_op E L v (v ◁ᵥ{π} n @ int it)%I (NotIntOp) (IntOp it) T.
