theories/caesium/notation.v
@@ -50,13 +50,6 @@ Notation "e1 ^{ ot1 , ot2 } e2" := (BinOp XorOp ot1 ot2 e1%E e2%E)
 Notation "e1 ,{ ot1 , ot2 } e2" := (BinOp Comma ot1 ot2 e1%E e2%E)
   (at level 30, format "e1  ,{ ot1 ,  ot2 }  e2") : expr_scope.
 
-Notation "e1 '+c' '{' ot1 , ot2 } e2" := (BinOp CheckedAddOp ot1 ot2 e1%E e2%E)
-  (at level 50, left associativity, format "e1  '+c' '{' ot1 ,  ot2 }  e2") : expr_scope.
-Notation "e1 '-c' '{' ot1 , ot2 } e2" := (BinOp CheckedSubOp ot1 ot2 e1%E e2%E)
-  (at level 50, left associativity, format "e1  '-c' '{' ot1 ,  ot2 }  e2") : expr_scope.
-Notation "e1 '×c{' ot1 , ot2 } e2" := (BinOp CheckedMulOp ot1 ot2 e1%E e2%E)
-  (at level 50, left associativity, format "e1  '×c{' ot1 ,  ot2 }  e2") : expr_scope.
-
 (* The offset must be evaluated first for the type system to work, thus the order is switched here. *)
 Notation "e1 'at_offset{' ly , ot1 , ot2 } e2" := (BinOp (PtrOffsetOp ly) ot2 ot1 e2%E e1%E)
   (at level 70, format "e1  at_offset{ ly ,  ot1 ,  ot2 }  e2") : expr_scope.
